progs/verif_incr.v
@@ -83,14 +83,12 @@ Proof.
   start_function.
   forward.
   forward_call (lock, sh, cptr_lock_inv ctr).
-  { apply prop_right; rewrite sem_cast_neutral_ptr; rewrite sem_cast_neutral_ptr; auto. }
   unfold cptr_lock_inv at 2; simpl.
   Intro z.
   forward.
   forward.
   rewrite field_at_isptr; Intros.
   forward_call (lock, sh, cptr_lock_inv ctr).
-  { apply prop_right; rewrite sem_cast_neutral_ptr; rewrite sem_cast_neutral_ptr; auto. }
   { lock_props.
     unfold cptr_lock_inv; Exists (z + 1); entailer!. }
   forward.
@@ -100,13 +98,11 @@ Lemma body_read : semax_body Vprog Gprog f_read read_spec.
 Proof.
   start_function.
   forward_call (lock, sh, cptr_lock_inv ctr).
-  { apply prop_right; rewrite sem_cast_neutral_ptr; rewrite sem_cast_neutral_ptr; auto. }
   unfold cptr_lock_inv at 2; simpl.
   Intro z.
   forward.
   rewrite data_at_isptr; Intros.
   forward_call (lock, sh, cptr_lock_inv ctr).
-  { apply prop_right; rewrite sem_cast_neutral_ptr; rewrite sem_cast_neutral_ptr; auto. }
   { lock_props.
     unfold cptr_lock_inv; Exists z; entailer!. }
   forward.
@@ -120,7 +116,6 @@ Proof.
   forward.
   forward_call (ctr, sh, lock).
   forward_call (lockt, sh, lock_inv sh lock (cptr_lock_inv ctr), thread_lock_inv sh ctr lock lockt).
-  { apply prop_right; rewrite sem_cast_neutral_ptr; rewrite sem_cast_neutral_ptr; auto. }
   { unfold thread_lock_inv; lock_props.
     rewrite selflock_eq at 2; cancel.
     eapply derives_trans; [apply lock_inv_later | cancel]. }
@@ -144,17 +139,14 @@ Proof.
   forward.
   forward.
   forward_call (lock, Ews, cptr_lock_inv ctr).
-  { apply prop_right; rewrite sem_cast_neutral_ptr; rewrite sem_cast_neutral_ptr; auto. }
   { rewrite (sepcon_comm _ (fold_right_sepcon _)); apply sepcon_derives; [cancel | apply lock_struct]. }
   rewrite field_at_isptr; Intros.
   forward_call (lock, Ews, cptr_lock_inv ctr).
-  { apply prop_right; rewrite sem_cast_neutral_ptr; rewrite sem_cast_neutral_ptr; auto. }
   { lock_props.
     unfold cptr_lock_inv; Exists 0; cancel. }
   (* need to split off shares for the locks here *)
   destruct split_Ews as (sh1 & sh2 & ? & ? & Hsh).
   forward_call (lockt, Ews, thread_lock_inv sh1 ctr lock lockt).
-  { apply prop_right; rewrite sem_cast_neutral_ptr; rewrite sem_cast_neutral_ptr; auto. }
   { rewrite (sepcon_comm _ (fold_right_sepcon _)); apply sepcon_derives; [cancel | apply lock_struct]. }
   get_global_function'' _thread_func.
   apply extract_exists_pre; intros f_.
@@ -178,13 +170,10 @@ Proof.
     entailer!. }
   forward_call (ctr, sh2, lock).
   forward_call (lockt, sh2, thread_lock_inv sh1 ctr lock lockt).
-  { apply prop_right; rewrite sem_cast_neutral_ptr; rewrite sem_cast_neutral_ptr; auto. }
   forward_call (ctr, sh2, lock).
   Intro z.
   forward_call (lock, sh2, cptr_lock_inv ctr).
-  { apply prop_right; rewrite sem_cast_neutral_ptr; rewrite sem_cast_neutral_ptr; auto. }
   forward_call (lockt, Ews, sh1, |>lock_inv sh1 lock (cptr_lock_inv ctr), |>thread_lock_inv sh1 ctr lock lockt).
-  { apply prop_right; rewrite sem_cast_neutral_ptr; rewrite sem_cast_neutral_ptr; auto. }
   { unfold thread_lock_inv; lock_props.
     - apply later_positive; auto.
     - unfold rec_inv.
@@ -196,7 +185,6 @@ Proof.
       rewrite sepcon_comm, <- !sepcon_assoc, sepcon_comm.
       apply sepcon_derives; [apply lock_inv_later | cancel]. }
   forward_call (lock, Ews, cptr_lock_inv ctr).
-  { apply prop_right; rewrite sem_cast_neutral_ptr; rewrite sem_cast_neutral_ptr; auto. }
   { lock_props.
     erewrite sepcon_assoc, lock_inv_share_join; eauto; cancel. }
   forward.
